monads: refactor Monad with functor.

monads/Monad.v
@@ -9,17 +9,30 @@ Module Type Monad.
   (** ">>=" *)
   Parameter bind : forall (A B : Type), m A -> (A -> m B) -> m B.
 
+  Infix ">>=" := bind (at level 50, left associativity).
+
   (** Three laws that a monad instance must obey.
     Law 1:  return x >>= f ~ f x
     Law 2:  m >>= return ~ m
     Law 3:  (m >>= f) >>= g ~ m >>= (fun x -> f x >>= g) *)
   Axiom monad_law1 : forall (A B : Type) (x : A) (f : A -> m B),
-    bind (ret x) f = f x.
+    ret x >>= f = f x.
 
   Axiom monad_law2 : forall (A : Type) (x : m A),
-    bind x (@ret A) = x.
+    x >>= @ret A = x.
 
   Axiom monad_law3 :
     forall (A B C : Type) (n : m A) (f : A -> m B) (g : B -> m C),
-      bind (bind n f) g = bind n (fun x => bind (f x) g).
+      (n >>= f) >>= g = n >>= (fun x => f x >>= g).
 End Monad.
+
+(** Functor of Monad with some extensions. *)
+Module MonadExt (M : Monad).
+  Import M.
+
+  Definition fmap (A B : Type) (f : A -> B) (n : m A) : m B :=
+    n >>= (fun x => ret (f x)).
+
+  Definition join (A : Type) (n : m (m A)) : m A :=
+    n >>= (fun x => x).
+End MonadExt.
